---
title: Chapter3-02. Sufficinecy and completeness
book_title: Mathematical statistics
book_chapter: 3
book_section: 2
---

## 3.2 Sufficinecy and completeness

### 3.2 Sufficient statistics
* $(\mathcal{X}, \mathcal{A})$,
    * measurable sp.
* $(\mathcal{T}, \mathcal{B})$,
    * measurable sp.
* $$\Theta \subseteq \mathbb{R}$$,
* $$\mathcal{P} := \{P_{\theta}\}_{\theta \in \Theta}$$,
    * family of measure over $(\mathcal{X}, \mathcal{A})$,
* $T: \mathcal{X} \rightarrow \mathcal{T}$
    * statistics

$T$ is said to be sufficient if

$$
    \forall A \in \mathcal{A},
    \
    \exists q_{A}:\mathcal{T} \rightarrow \mathbb{R}: \mathcal{B} \text{-measurable }
    \
    \text{ s.t. }
    \
    \forall B \in \mathcal{B},
    \
    \theta \in \Theta,
    \
    \int_{B}
        q_{A}(t)
    \ d P_{\theta}^{T}(dt)
    =
    P_{\theta}(A \cap T^{-1}(B))
$$

<div class="end-of-statement" style="text-align: right">■</div>

### Remark
The definition of sufficiency is interpreted as the family of distributions can be expressed by the measurable funciton which does not depend on $\theta$.
In other words, a statistics $T$ has **sufficient** information to determine a $\theta$.
The definition of sufficient statistics is equivalent to

$$
    \forall A \in \mathcal{A},
    \
    \exists q_{A}: \mathcal{T} \rightarrow \mathbb{R}: \mathcal{B} \text{-measurable }
    \
    \text{ s.t. }
    \
    q_{A}(t)
    =
    P_{\theta}(A \mid T = t)
    \
    t \text{-a.e.}
$$

<div class="end-of-statement" style="text-align: right">■</div>

### Example 3.1 Bernoulli trial
* $$\mathcal{X} := \{0, 1\}^{n}$$,
* $$\mathcal{A} := 2^{\mathcal{X}}$$,
* $$\Theta := [0, 1]$$,
* $$\mathcal{T} := \{0, 1, \ldots, n\}$$,
* $$\mathcal{B} := 2^{\mathcal{T}}$$,

We define p.d.f. of this trials as follows.

$$
    \theta \in \Theta,
    \
    x \in \mathcal{X},
    \
    p_{\theta}(x)
    :=
    \theta^{\sum_{i=1}^{n} x_{i}}
    (1 - \theta)^{n - \sum_{i=1}^{n} x_{i}},
$$

Corresponding probability measure is

$$
    A \in \mathcal{A}
    \
    P_{\theta}(A)
    :=
    \sum_{x \in A}
        p_{\theta}(x).
$$

We show that statistic

$$
    T(x)
    :=
    \sum_{i=1}^{n}
        x_{i}
$$

is sufficient.
To show that, we need to confirm the equation of definition of sufficiency.
It is easy to see that

$$
\begin{eqnarray}
    P_{\theta}(\{x\} \cap T^{-1}(\{t\})
    =
    \begin{cases}
        \theta^{t}(1 - \theta)^{n - t}
        &
            x \in T^{-1}(\{t\})
            \\
        0
        &
            x \notin T^{-1}(\{t\})
    \end{cases}.
    \label{example_sufficiency_lhs}
\end{eqnarray}
$$

Hence

$$
\begin{eqnarray}
    \forall A \in \mathcal{A},
    \
    P_{\theta}(A \cap T^{-1}(\{t\})
    & = &
        P_{\theta}(A \cap T^{-1}(\{t\}))
    \nonumber
    \\
    & = &
        \sum_{x \in A}
            P_{\theta}(\{x\} \cap T^{-1}(\{t\}))
    \nonumber
    \\
    & = &
        |A \cap T^{-1}(\{t\}) |
            \theta^{t}(1 - \theta)^{n - t}.
    \nonumber
\end{eqnarray}
$$

In particular, if we take $A$ as $\mathcal{X}$, we have

$$
\begin{eqnarray}
    P_{\theta}(T^{-1}(\{t\})
    & = &
        |T^{-1}(\{t\}) |
            \theta^{t}(1 - \theta)^{n - t}.
    \nonumber
    \\
    & = &
        |\{x \in \mathcal{X} \mid \sum_{i=1}^{n} x_{i} = t \} |
            \theta^{t}(1 - \theta)^{n - t}.
    \nonumber
    \\
    & = &
        \left(
            \begin{array}{c}
                n \\
                t
            \end{array}
        \right)
            \theta^{t}(1 - \theta)^{n - t}.
    \nonumber
\end{eqnarray}
$$

For evey $A$  we define $\mathcal{B}$ measurable function $$q_{A}$$ by

$$
\begin{eqnarray}
    r(x, t)
    :=
    \begin{cases}
        \left(
            \begin{array}{c}
                n \\
                t
            \end{array}
        \right)^{-1}
        &
            (T(x) = t)
        \\
        0
        &
            \text{otherwise}
    \end{cases}
    \nonumber
\end{eqnarray}
$$

$$
    q_{A}(t)
    :=
    \sum_{x \in A}
        r(x, t)
    =
    |A \cap T^{-1}(\{t\})|
        \left(
            \begin{array}{c}
                n \\
                t
            \end{array}
        \right)^{-1}
$$

Now we show that $$q_{A}$$ satisfies the equality of the definition of sufficiency.
LHS of the equality is

$$
\begin{eqnarray}
    \int_{B}
        q_{A}(t)
    P_{\theta}^{T}(dt)
    & = &
        \sum_{t \in B}
            q_{A}(t)
            P_{\theta}^{T}(\{t\})
    \nonumber
    \\
    & = &
        \sum_{t \in B}
            q_{A}(t)
            \left(
                \begin{array}{c}
                    n \\
                    t
                \end{array}
            \right)
                \theta^{t}(1 - \theta)^{n - t}.
    \nonumber
    \\
    & = &
        \sum_{t \in B}
            |A \cap T^{-1}(\{t\})|
            \theta^{t}(1 - \theta)^{n - t}.
    \nonumber
\end{eqnarray}
$$

RHS of the equality is

$$
\begin{eqnarray}
    P_{\theta}(A \cap T^{-1}(B))
    & = &
        \sum_{t \in B}
            P_{\theta}(A \cap T^{-1}(\{t\}))
    \nonumber
    \\
    & = &
        \sum_{t \in B}
            |A \cap T^{-1}(\{t\}) |
                \theta^{t}(1 - \theta)^{n - t}.
\end{eqnarray}
$$

<div class="end-of-statement" style="text-align: right">■</div>

### Proposition 3.3
* $$\{P_{\theta}\}_{\theta \in \Theta}$$,
* $f: \mathcal{X} \rightarrow \mathbb{R}$,
    * measurable
    * for all $\theta \in \Theta$, $P_{\theta}$-integrable
* $T: \mathcal{X} \rightarrow \mathcal{T}$,
    * sufficient statistics

Then there exists measurable function $g:\mathcal{T} \rightarrow \mathbb{R}$l such that

$$
    \forall \theta \in \Theta,
    \
    g(t)
    =
    \mathrm{E}_{\theta}
    \left[
        f
        \mid
        T = t
    \right]
    \quad
    P_{\theta}^{T}\text{-a.s.}
$$

### proof

<div class="QED" style="text-align: right">$\Box$</div>

### Definition 3.11 Complete
* $(\mathcal{X}, \mathcal{A})$,
    * measurable space
* $\Theta$
    * parameter sp.
* $\{P_{\theta}\}_{\theta \in \Theta}$
    * a family of probability distribution over $(\mathcal{X}, \mathcal{A})$.

$\mathcal{P}$ is said to be (boundedly) complete if for all (bounded) measurable function $f: \mathcal{X} \rightarrow \mathbb{R}$,

$$
\begin{eqnarray}
    \mathrm{E}_{\theta}
    \left[
        f
    \right]
    =
    0
    \
    (\forall \theta \in \Theta)
    \
    \Rightarrow
    \
    \forall \theta \in \Theta
    f = 0
    \
    P_{\theta} \text{-a.s.}
    ,
\end{eqnarray}
$$

<div class="end-of-statement" style="text-align: right">■</div>

### Remark
If $f \ge 0$, the above statemet always holds.

<div class="end-of-statement" style="text-align: right">■</div>

### Definition 3.12 complete map
* $(\mathcal{T}, \mathcal{B})$,
    * measurable sp.
* $f: \mathcal{X} \rightarrow \mathcal{T}$,
    * measurable map

$T$ is said to be (boundedly) complete if $$\{P_{\theta}^{T}\}_{\theta \in \Theta}$$ is (boundedly) complete.

<div class="end-of-statement" style="text-align: right">■</div>

### Proposition 3.3
* $$\mathcal{P} := \{P_{\theta}\}_{\theta \in \Theta}$$,
* $f: \mathcal{X} \rightarrow \mathbb{R}$,
    * $\forall \theta \in \Theta$, $P_{\theta}$-integrable
* $T: \mathcal{X} \rightarrow \mathbb{R}$,
    * sufficient with respect to $\mathcal{P}$,

Then there exists measurable function $g: \mathcal{T} \rightarrow \mathbb{R}$ such that

$$
    \forall \theta \in \Theta,
    \
    g(t)
    =
    \mathrm{E}_{\theta}
    \left[
        f
        \mid
        T = t
    \right]
    \quad
    P_{\theta}^{T} \text{-a.s.}
$$

### proof

<div class="QED" style="text-align: right">$\Box$</div>

### Proposition 3.4
* $$\mathcal{P} := \{P_{\theta}\}_{\theta \in \Theta}$$,
* $f: \mathcal{X} \rightarrow \mathbb{R}$,
    * $\forall \theta \in \Theta$, $P_{\theta}$-integrable
* $T: \mathcal{X} \rightarrow \mathbb{R}$,
    * sufficient with respect to $\mathcal{P}$,

Then there exists $f^{\prime}: \mathcal{X} \rightarrow \mathbb{R}$ such that

$$
    \forall \theta \in \Theta,
    \
    f^{\prime}(x)
    =
    \mathrm{E}_{\theta}
    \left[
        f
        \mid
        T
    \right]
    \quad
    P_{\theta} \text{-a.s.}
$$

### proof

<div class="QED" style="text-align: right">$\Box$</div>
