---
title: Chapter3-04. Distributions with Monotone Likelihood Ratio
book_title: Testing Statistical Hypotheses
book_chapter: 3
book_section: 4
---

## 3.4 Distributions with Monotone Likelihood Ratio

### Definition (Monotone Likelihood Ration)
We  say that $(p_{\theta})_{\theta \in \Theta}$ have monotone likelihood ration if

$$
    \exists T: \mathcal{X} \rightarrow \mathbb{R}: \text{measurable}
    \quad
    \text{ s.t. }
    \
    \forall \theta < \theta^{\prime},
    \
    \exists g: \mathbb{R} \rightarrow \mathbb{R}_{\ge 0}: \text{non-deceasing},\
    \
    \frac{
        p_{\theta^{\prime}}(x)
    }{
        p_{\theta}(x)
    }
    =
    g(T(x))
    \quad
    (\forall x \in \mathcal{X})
    .
$$

<div class="end-of-statement" style="text-align: right">■</div>

### Theorem 3.4.1
* $(p_{\theta})_{\theta \in \Theta}$,
    * with MLR in $T$

* (i) Let $\theta_{0} \in \Theta$ be fixed and considered the hypothesis $$\Theta_{0} := \{\theta \mid \theta \le \theta_{0}\}$$ and alternatives $$\Theta_{1} := \{\theta \mid \theta_{0} < \theta\}$$. $\forall \alpha \in (0, 1)$, there exists UMP test $\phi$ defined by

$$
    \phi(x)
    :=
    \begin{cases}
        1
        &
            (T(x) > C)
        \\
        \gamma
        &
            (T(x) = C)
        \\
        0
        &
            (T(x) < C)
    \end{cases}
$$

where $\gamma$ and $C$ are consntats.

$$
    \beta_{\phi}(\theta_{0})
    =
    \alpha
$$

* (ii) $\beta_{\phi}(\theta)$ is non-deacreasing in $\theta \in \Theta$.
Moreover, $\beta_{\phi}(\theta)$ is stricty increasing in $\theta \in \beta_{\phi}^{-1}((0, 1))$.

* (iii) For $\forall \theta^{\prime} \in \Theta$, $\phi$ gives the UMP test for the hypothesis $$\Theta_{0} := \{\theta \mid \theta \le \theta^{\prime}\}$$ and alternatives $$\Theta_{1} := \{\theta \mid \theta^{\prime} < \theta\}$$ at level $\alpha^{\prime} := \beta_{\phi}(\theta^{\prime})$.

* (iv) 

$$
    \phi
    =
    \argmin_{\phi^{\prime}}
        \{
            \beta_{\phi^{\prime}}(\theta)
            \mid
            \theta < \theta_{0},
            \
            \beta_{\phi^{\prime}}(\theta)
        \}
$$

### proof
(i), (ii)

It suffices to show that $\exists C, \gamma$ such that

$$
\begin{eqnarray}
    & &
        \mathrm{E}_{\theta_{0}}
        \left[
            \phi(X)
        \right]
        =
        \alpha
    \nonumber
    \\
    & \Leftrightarrow &
        P_{\theta_{0}}(T(X) > C)
        +
        \gamma P_{\theta_{0}}(T(X) = C)
        =
        \alpha
    \nonumber
\end{eqnarray}
$$

Let us defined

$$
    \phi(C)
    :=
    P_{\theta_{0}}(T(X) = C)
    \quad
    (C \in \mathbb{R})
    .
$$

Thus, $\phi$ is right continuous with left limits and

$$
    \phi(-\infty) = 0,
    \
    \phi(\infty) = 1,
    .
$$

Since

$$
\begin{eqnarray}
    P_{\theta_{0}}(T(X) > C)
    & = &
        1 - \phi(C)
    \nonumber
    \\
    P_{\theta_{0}}(T(X) = C)
    & = &
        \Delta \phi(C)
    \nonumber
\end{eqnarray}
$$

where $$\Delta \phi(C) := \phi(C) - \phi(C-)$$.

$$
\begin{eqnarray}
    & &
        1 - \phi(C) + \gamma \Delta \phi(C)
        =
        \alpha
    \nonumber
    \\
    & \Leftrightarrow &
        \phi(C)
        =
        1 - \alpha + \gamma \Delta \phi(C)
    \nonumber
\end{eqnarray}
$$

Hence let

$$
    C^{*}
    :=
    \inf
        \{
            C
            \mid
            \phi(C)
            \ge
            1 - \alpha
        \}
    \in \mathbb{R}
    .
$$

Then by right continutity, we have

$$
    \phi(C^{*})
    \ge
    1 - \alpha
    .
$$

In case of $\phi(C^{*}) = 1- \alpha$,

$$
    \gamma^{*}
    :=
    0
    .
$$

In case of $$\phi(C^{*}) > 1 - \alpha$$, $C^{*}$ is a 
Indeed,

Take any $$C < C^{*}$$.
Then by definition of $C^{*}$ we have

$$
    \phi(C) < 1 - \alpha.
$$

$$
\begin{eqnarray}
    \phi(C^{*}-)
    & = &
        \lim_{C \nearrow C^{*}} 
            \phi(C)
    \nonumber
    \\
    & \ge &
        1 - \alpha
    \nonumber
    \\
    & < &
        \phi(C)
    .
    \nonumber
\end{eqnarray}
$$

Therefore 

$$
    \phi(C^{*}-) \le 1 - \alpha < \phi(C^{*})
    .
$$

Let us defined $\gamma^{*}$ by

$$
    \gamma^{*}
    :=
    \frac{
        \phi(C^{*}) - (1 - \alpha)
    }{
        \Delta \phi(C^{*})
    }
    \in [0, 1]
    .
$$

proof of (ii)

Let $\theta^{\prime} < \theta^{\prime\prime}$.
Then consider $\phi^{\prime}$ such that

$$
    \phi^{\prime}
    \equiv
    \alpha^{\prime}
    =
    \beta_{\phi}(\theta^{\prime})
    \in (0, 1)
    .
$$

Then it follow that

$$
\begin{eqnarray}
    & &
        \beta_{\phi^{\prime}}(\theta^{\prime\prime})
        \ge
        \beta_{\phi}(\theta^{\prime\prime})
    \nonumber
    \\
    & \Leftrightarrow &
        \beta_{\phi^{\prime}}(\theta^{\prime})
        \ge
        \beta_{\phi}(\theta^{\prime\prime})
    \nonumber
\end{eqnarray}
$$

Assume $\beta_{\phi}(\theta^{\prme\prime}) = \beta_{\phi}(\theta^{\prime\prime})$.


<div class="QED" style="text-align: right">$\Box$</div>

### Lemma
* $\theta^{\prime}$ < \theta^{\prime\prime}$,
* $\alpha^{\prime} := \beta_{\phi}(\theta^{\prime})$,

$\phi$ is MP test at levelt $\alpha^{\prime}$ for hypothesis $$\Theta_{0} := \{P_{\theta^{\prime}}\}$$ and alternatives $$\Theta_{1} := \{P_{\theta^{\prime\prime}}\}$$.

### proof
By MLR, there exists non decreasing function $g: \mathbb{R} \rightarrow \mathbb{R}$ such that

$$
    g(T(x))
    =
    p_{\theta^{\prime\prime}}(x)
    \frac{
        p_{\theta^{\prime\prime}}(x)
    }{
        p_{\theta^{\prime}}(x)
    }
    .
$$

Using $g$, $\phi$ satisfy

$$
    \phi(x)
    =
    \begin{cases}
        1
        &
            (p_{\theta^{\prime\prime}}(x) > k p_{\theta^{\prime}}(x))
        \\
        0
        &
            (p_{\theta^{\prime\prime}}(x) > k p_{\theta^{\prime}}(x))
    \end{cases}
$$

where $k := g(C)$.

$$
\begin{eqnarray}
    & &
        \Gamma(x) > c
    \nonumber
    \\
    & \Leftrightarrow &
        g(T(x)) > g(C)
    \nonumber
    \\
    & \Leftrightarrow &
        p_{\theta^{\prime\prime}}(x)
        >
        g(C)p_{\theta^{\prime}}(x)
    \nonumber
\end{eqnarray}
$$

<div class="QED" style="text-align: right">$\Box$</div>



### Definition Essentially complete
* $C \subseteq \Phi$,

$C$ is said to be essentially complete if

$$
    \forall \phi \in \Phi \setminus C,
    \
    \exists \phi^{\prime} \in C,
    \
    \forall \theta \in \Theta,
    \
    R(\theta, \phi)
    \ge 
    R(\theta, \phi^{\prime})
    .
$$

<div class="end-of-statement" style="text-align: right">■</div>

* $L_{0}: \Theta \rightarrow \mathbb{R}$,
    * strictly increasing in $\theta \ge \theta_{0}$
* $L_{1}: \Theta \rightarrow \mathbb{R}$,
    * decreasing increasing for $\theta \le \theta_{0}$

$$
    L_{1}(\theta)
    -
    L_{0}(\theta)
    \begin{cases}
        >
        0
        &
            \theta < \theta_{0}
        \\
        <
        0
        &
            \theta > \theta_{0}
    \end{cases}
$$

### Theorem 3.4.2
* $\Theta \subseteq \mathbb{R}$,
* $\theta_{0} \in \Theta$,
* $L: \Theta \times \mathcal{X} \rightarrow \mathbb{R}$,

$$
    \mathcal{C}
    :=
    \{
        \phi: \mathcal{X} \rightarrow [0, 1]
        \mid
        \forall \alpha \in [0, 1],
        \
        \phi
        \text{ satisfies}
        \eqref{chap03_03_16},
        \eqref{chap03_03_17}.
    \}
$$

* (i) $\mathcal{C}$ is essentially complete.
* (ii) $\mathcal{C}$ is minimal essentially complete if

$$
    \forall \theta, \theta^{\prime} \in \Theta,
    \
    \{
        x \in \mathcal{X}
        \mid
        p_{\theta}(x) > 0
    \}
    =
    \{
        x \in \mathcal{X}
        \mid
        p_{\theta^{\prime}}(x) > 0
    \}
    .
$$

### proof
(i)

$$
\begin{eqnarray}
    R(\theta, \phi)
    & = &
        \int_{\mathcal{X}}
            p_{\theta}(x)
            \left(
                \phi(x)
                L_{1}(\theta)
                +
                (1 - \phi(x))
                L_{0}(\theta)
            \right)
        \ \mu(dx)
    \nonumber
    \\
    & = &
        \int_{\mathcal{X}}
            p_{\theta}(x)
            \left(
                L_{0}(\theta)
                +
                (L_{1}(\theta) - L_{0}(\theta))
                \phi(x)
            \right)
        \ \mu(dx)
    \nonumber
\end{eqnarray}
$$

Hence

$$
\begin{eqnarray}
    R(\theta, \phi^{\prime})
    -
    R(\theta, \phi)
    & = &
        (L_{1}(\theta) - L_{0}(\theta))
        \int_{\mathcal{X}}
            (\phi^{\prime}(x) - \phi(x))
            p_{\theta}(x)
        \ \mu(dx)
    \nonumber
\end{eqnarray}
$$

If

$$
\begin{eqnarray}
    \beta_{\phi^{\prime}}(\theta)
    -
    \beta_{\phi}(\theta)
    & = &
        \int_{\mathcal{X}}
            (\phi^{\prime}(x) - \phi(x))
            p_{\theta}(x)
        \ \mu(dx)
    & &
        \begin{cases}
            >
            0
            &
                (\theta > \theta_{0})
            \\
            <
            0
            &
                (\theta < \theta_{0})
            \\
            =
            0
            &
                (\theta = \theta_{0})
        \end{cases},
    \nonumber
\end{eqnarray}
$$

then

$$
    \forall \theta \in \Theta,
    \
    R(\theta, \phi^{\prime})
    -
    R(\theta, \phi)
    \le
    0
    .
$$

<div class="QED" style="text-align: right">$\Box$</div>


