---
title: Chapter3. Probability measure
book_title: Optimization in Function Spaces with stability considerations in Orlicz Spaces
book_chapter: 3
book_section: 11
---
## 3.11 Conjugate Functions


### Definition 3.11.1
* $X$
    * norm space
* $$f: X \rightarrow real_number \cup \{\infty\}$$,
* $\mathrm{Dom}f \neq \emptyset$,

The conjugate function $$f^{*}: X^{*} \rightarrow \mathbb{R} \cup \{\infty\}$$ is defined by

$$
    f^{*}(y)
    :=
    \sup
    \{
        \langle y, x \rangle
        -
        f(x)
        \mid
        x \in X
    \}
    .
$$

$f^{*}$ is also called the dual of $f$.

<div class="end-of-statement" style="text-align: right">â– </div>

### Remark
The supremum of set of convex functions is also convex.
It follows that $f^{*}$ is convex if $f$ is convex.
Moreover Yong's inequality holds;

$$
\begin{equation}
    \forall x \in X,
    \
    \forall y \in X^{*},
    \
    \langle x, y \rangle
    \le
    f(x)
    +
    f^{*}(y)
    .
    \label{chap03_03_15}
\end{equation}
$$

<div class="QED" style="text-align: right">$\Box$</div>

### Theorem 3.11.2
* $X$
    * norm space
* $$f:X \rightarrow \mathbb{R} \cup \{\infty\}$$,
* $\partial f(x) \neq \emptyset$,

Following statements are equavalent:

* (1)

$$
    \forall y \in X^{*},
    \
    f(x) + f(y)
    =
    \langle x, y \rangle
    .
$$

* (2) $y \in \partial f(x)$.

### proof
(1) $\Rightarrow$ (2)

Let $x \in X$ be fixed.

$$
\begin{eqnarray}
    \forall u \in X,
    \
    \langle u, y \rangle
    & \le &
        f(u)
        +
        f^{*}(y)
    \nonumber
    \\
    \langle u, y \rangle
    & \le &
        f(u)
        +
        \langle x, y \rangle
        -
        f(x)
    \nonumber
    \\
    \langle u - x, y \rangle
    & \le &
        f(u)
        -
        f(x)
    .
\end{eqnarray}
$$

Hence $y \in \partial f(x)$.

(1) $\Leftarrow$ (2)

Let $y \in \partial f(x)$.

$$
\begin{eqnarray}
    \forall z \in X,
    \
    f(z) - f(x)
    & \ge &
        \langle z - x, y \rangle
    \nonumber
    \\
    \langle x, y \rangle
     - f(x)
    & \ge &
        \langle z, y \rangle
        -
        f(z)
    \nonumber
\end{eqnarray}
$$

By taking supremum of RHS, we have

$$
    \langle x, y \rangle
     - f(x)
    \ge
    \sup
    \{
        \langle z, y \rangle
        -
        f(z)
        \mid
        z \in Z
    \}
    =
    f^{*}(y)
    .
$$

<div class="QED" style="text-align: right">$\Box$</div>

### Lemma 3.11.3
* $X$
    * norm space
* $f: X \rightarrow \bar{\mathbb{R}}$,
    * l.s.c. convex

$f$ has an affine minorant, that is,

$$
    \forall x \in \mathrm{Dom}f,
    \
    d > 0,
    \
    \exists z \in X^{*}
    \text{ s.t. }
    \forall y \in X,
    \
    f(y)
    >
    f(x)
    +
    \langle y - x, z \rangle
    -
    d
    .
$$

### proof


<div class="QED" style="text-align: right">$\Box$</div>
