---
title: Chapter3. Inner space and Hilbert space
book_title: Functional Analysis
book_chapter: 3
book_section: 4
---

## 3.4 Riesz's representer theorem


### Definition linear functional
* $K = \mathbb{R}, \mathbb{C}$
    * field
* $X$
    * linear space over $K$
* $f:X \rightarrow K$

$f$ is said to be linear function if 

$$
\begin{eqnarray}
    f(u + v)
    & = &
        f(u) + f(v)
    & &
        (u, v \in X),
    \nonumber
    \\
    f(\alpha u)
    & = &
        \alpha f(u)
    & &
        (\alpha \in K, u \in X)
    .
    \nonumber
\end{eqnarray}
$$

<div class="end-of-statement" style="text-align: right">■</div>

### Definition 3.7 dual space
* $X$
    * topological linear space,

We denote $$X^{*}$$ by a set of continuous linear functionals over $X$.
$$X^{*}$$ is called dual space.

<div class="end-of-statement" style="text-align: right">■</div>

### Remark
$X^{*}$ is a linear space over $K$.
Indeed, we define operations as follows:

$$
\begin{eqnarray}
    (f + g)(u)
    & \Leftrightarrow &
        f(u)
        +
        g(u)
    & &
        (u \in X)
    \nonumber
    \\
    (\alpha f)(u)
    & = &
        \alpha f(u)
    & &
        (u \in X)
        .
    \nonumber
\end{eqnarray}
$$

<div class="end-of-statement" style="text-align: right">■</div>

### Definition 3.8 boundedness of linear functionals
* $X$,
    * norm space
* $f:X \rightarrow K$,
    * linear functional

$f$ is said to be bounded if

$$
\begin{equation}
    \exists M \in \mathbb{R},
    \
    \text{ s.t. }
    \
    \forall u \in X,
    \
    |f(u)|
    \le
    M \| u \|
    \label{chap03_04_03_36_boundedness}
    .
\end{equation}
$$

<div class="end-of-statement" style="text-align: right">■</div>

### Theorem 3.4
* $X$
    * norm space
* $f: X \rightarrow K$,
    * linear functional

$f$ is continuous if and only if $f$ is bounded.

### proof
We first show if part.
Suppose that $$\eqref{chap03_04_03_36_boundedness}$$ holds.
Then, if $$u_{n} \rightarrow u_{0} \ (n \rightarrow \infty)$$, we have

$$
\begin{eqnarray}
    |f(u_{n}) - f(u_{0})|
    & = &
        |f(u_{n} - u_{0})|
    & \le &
        M \|u_{n} - u_{0}\|
        \rightarrow
        0
    .
    \nonumber
\end{eqnarray}
$$

Hence $f$ is continuous.

We next show only if part.
Suppose that $f$ is not bounded.
There exists $$\{u_{n}\}$$ such that

$$
    \forall n \in \mathbb{N},
    \
    |f(u_{n})|
    >
    n \|u_{n}\|
    .
$$

Obviously $u_{n} \neq 0$.
Let

$$
    v_{n}
    :=
    \frac{
        u_{n}
    }{
        n \|u_{n} \|
    }
    .
$$

$$\|v_{n}\| = 1 / n \rightarrow 0$$, $v_{n} \rightarrow 0$.
Thefore, by continuity of $f$, we have

$$
    f(v_{n}) \rightarrow 0
    .
$$

However,

$$
    |f(v_{n})|
    =
    \left|
        f
        \left(
            \frac{
                u_{n}
            }{
                n \|u_{n}\|
            }
        \right)
    \right|
    >
    \frac{
        n \|u_{n}\|
    }{
        n \|u_{n}\|
    }
    =
    1
    .
$$

If we take the limit of both side of above equation, we have a contradiction.
Thefore, $f$ is bounded

<div class="QED" style="text-align: right">$\Box$</div>

### Definition 3.9 norm in dual space
* $X$,
    * norm space
* $f \in X^{*}$,

$$
    \|f\|_{X^{*}}
    :=
    \inf
    \{
        M \in \mathbb{R}
        \mid
        |f(u)|
        \le
        M \|u\|
        \quad
        (u \in X)
    \}.
$$

$$\|f\|_{X^{*}}$$ is called norm of $f$.

<div class="end-of-statement" style="text-align: right">■</div>

### Proposition

$$
\begin{eqnarray}
    \|f\|
    & = &
        \sup_{u \neq 0}
            \frac{
                |f(u)|
            }{
                \|u\|
            }
    & = &
        \sup_{\|v\| = 1}
            |f(v)|
    \nonumber
\end{eqnarray}
$$

### proof

$$
    \forall u \neq 0 \in X,
    \
    \frac{
        |f(u)|
    }{
        \|u\|
    }
    \le
    \frac{
        \|u\| \|f\|
    }{
        \|u\|
    }
    =
    \|f\|
    .
$$

Hence

$$
\begin{eqnarray}
    \sup_{u \neq 0}
        \frac{
            |f(u)|
        }{
            \|u\|
        }
    \le
    \|f\|
    .
\end{eqnarray}
$$

Conversely,

$$
    \forall u \in X,
    \
    |f(u)|
    \le
    |f(u)|
    \frac{
        \|u\|
    }{
        \|u\|
    }
    \le
    \sup_{u^{\prime} \neq 0}
        \frac{
            |f(u^{\prime})|
        }{
            \|u^{\prime}\|
        }
        \|u\|
    .
$$

Hence

$$
    \sup_{u \neq 0}
        \frac{
            |f(u)|
        }{
            \|u\|
        }
    \in
    \{
        M \in \mathbb{R}
        \mid
        |f(u)|
        \le
        M \|u\|
        \quad
        (u \in X)
    \}
    .
$$

It follows that

$$
\begin{eqnarray}
    \sup_{u \neq 0}
        \frac{
            |f(u)|
        }{
            \|u\|
        }
    \ge
    \|f\|
    .
\end{eqnarray}
$$

<div class="QED" style="text-align: right">$\Box$</div>

### Propostion
$$(X^{*}, \|\cdot\|_{X^{*}})$$ is norm space.

### proof

$$
    \sup_{\|v\| = 1}
        |(f + g)(v)|
    \le
    \sup_{\|v\| = 1}
        \left(
            |f(v)|
            +
            |g(v)|
        \right)
    \le
    \|f\|
    +
    \|g\|
    .
$$

$$
    \|\alpha f\|
    =
    \sup_{\| v\| = 1}
        |\alpha f(v)|
    =
    \sup_{\| v\| = 1}
        |\alpha| |f(v)|
    =
    |\alpha| 
    \|f\|
    .
$$

<div class="QED" style="text-align: right">$\Box$</div>

$$
    f \in X^{*},
    \
    N_{f}
    :=
    \mathrm{Ker}f
    =
    \{
        u \in X
        \mid
        f(u) = 0
    \}
$$

### Proposition 3.3
$N_{f}$ is closed subspace in $X$.

### proof
Closedness is obvious since $f$ is continuous.
Moreover, linearity is also obvious since $f$ is linear.

<div class="QED" style="text-align: right">$\Box$</div>

### Theorem Riesz's representor theorem
* $X$
    * Hilbert space

$$
\begin{equation}
    \forall f \in X^{*},
    \
    \exists ! a \in X,
    \
    \text{ s.t. }
    \
    f(u)
    =
    (u, a)
    \quad
    (u \in X)
    \label{chap03_04_03_44_riesz}
    .
\end{equation}
$$

### proof
Uniquness.

Suppose that $f(u) = (u, a_{1}) = (u, a_{2})$.
It follows that $(u, a_{1} - a_{2}) = 0$.
Hence $a_{1} - a_{2} = 0$.

Existence.

Let $N_{f} := \mathrm{Ker}f$.
If $N_{f} = X$, then $f \equiv 0$.
In this case, $a = 0$ satisfies the statement.
Now we assume $N_{f} \neq X$.
There exists $c \in X$ such that $c \notin N_{f}$.
Let $p \in N_{f}$ be orthogonal projection of $c$ and $b := c - p$.
Then we have

$$
\begin{eqnarray}
    f(b)
    & = &
        f(c - p)
        =
        f(c)
        \neq
        0
    \nonumber
    \\
    b
    & \perp &
        N_{f}
    \nonumber
    \\
    b
    & \neq &
        0
    \nonumber
\end{eqnarray}
$$

For $u \in X$, let

$$
\begin{eqnarray}
    \alpha(u)
    & := &
        \frac{
            f(u)
        }{
            f(b)
        }
    \nonumber
    \\
    w
    & := &
        u - \alpha(u)b
    .
    \nonumber
    \\
    f(w)
    & = &
        f(u) - \alpha(u)f(b)
        =
        0
    .
    \nonumber
\end{eqnarray}
$$

Hence $w \in N_{f}$.

$$
\begin{eqnarray}
    0
    & = &
        (w, b)
    \nonumber
    \\
    & = &
        (u, b)
        -
        \alpha(i)\|b\|^{2}
    \nonumber
    \\
    & = &
        (u, b)
        -
        \frac{
            f(u)
        }{
            f(b)
        }
        \|b\|^{2}
    .
\end{eqnarray}
$$

Therefore, we have


$$
    f(u)
    =
    \left(
        u,
        \frac{
            \overline{f(u)}
        }{
            \|b\|^{2}
        }
        b
    \right)
    .
$$

It follows that $a := \overline{f(b)}b/\|b\|^{2}$ satisfies the statement.

<div class="QED" style="text-align: right">$\Box$</div>

For $f \in X^{*}$, we denote $Jf$ by $a$ in $$\eqref{chap03_04_03_44_riesz}$$ corresponding to $f$.
With this notation,

$$
\begin{equation}
    f(u)
    =
    (u, Jf)
    \quad
    (u \in X)
    .
    \label{chap03_04_03_47}
\end{equation}
$$

$J:X^{*} \rightarrow X$ is isometric, that is,

$$
\begin{equation}
    \|Jf\|_{X}
    =
    \|f\|_{X^{*}}
    .
    \label{chap03_04_03_48}
\end{equation}
$$

Indeed,

$$
\begin{equation}
    \forall u \in X,
    \
    |f(u)|
    =
    |(u, Jf)|
    \le
    \|u\|
    \|Jf\|
    \label{chap03_04_03_49}
    .
\end{equation}
$$

Moreover,

$$
    |f(Jf)|
    =
    |(Jf, Jf)|
    =
    \|Jf\|^{2}
    .
$$

It follows that the equality $$\eqref{chap03_04_03_49}$$ holds when $u := Jf$.
When $Jf \neq 0$,

$$
    \|f\|
    =
    \sup_{u \neq 0}
        \frac{
            |f(u)|
        }{
            \|u\|
        }
    =
    |Jf|
    .
$$

In case of $Jf = 0$, we have

$$
    |f(u)|
    \le
    \|Jf\|
    \|u\|
    =
    0
    .
$$

Since $f \equiv 0$, 

$$
    \|Jf\|
    =
    \|f\|
    =
    0
    .
$$

